src/parse/Castor.v
@@ -1,0 +1,28 @@
+From Pollux Require Import Prelude.
+From Pollux.parse Require Import Util.
+From Pollux.parse Require Import Input.
+From Pollux.parse Require Import Result.
+From Pollux.parse Require Import Parser.
+From Pollux.parse Require Import Serializer.
+From Pollux.parse Require Import Theorems.
+From Pollux.parse Require Import TheoremsRel.
+
+From Corelib.Program Require Import Basics Tactics.
+From Stdlib.Program Require Import Program.
+
+Module Castor (Input : AbstractInput).
+  Declare Module R : Result Input.
+  Declare Module Parser : Parser Input R.
+  Declare Module Serializer : Serializer Input R.
+  Declare Module T : Theorems Input R Parser Serializer with Module S := Serializer with Module P := Parser.
+  Declare Module TR : TheoremsRel Input R Parser Serializer T.
+
+  Import Input.
+  Export Input.
+  Import R.
+  Export R.
+  Import T.
+  Export T.
+  Import TR.
+  Export TR.
+End Castor.
